opentheory/examples/probability.ml
@@ -95,63 +95,70 @@ let rdecode_list_def = new_definition
 
 export_thm rdecode_list_def;;
 
-(***
-let rdecode_uniform_dest_def =
- (`!n r.
+let (rdecode_uniform_dest_zero,rdecode_uniform_dest_suc) =
+  let def = new_recursive_definition num_RECURSION
+    `(!r. rdecode_uniform_dest 0 r = (0,r)) /\
+     (!r w.
+        rdecode_uniform_dest (SUC w) r =
+        let (b,r') = rbit r in
+        let (m,r'') = rdecode_uniform_dest w r' in
+        ((if b then 2 * m + 1 else 2 * m), r''))` in
+  CONJ_PAIR def;;
+
+export_thm rdecode_uniform_dest_zero;;
+export_thm rdecode_uniform_dest_suc;;
+
+let rdecode_uniform_dest_def = CONJ rdecode_uniform_dest_zero rbits_suc;;
 
 let rdecode_uniform_loop_exists = prove
- (`!d. ?dest. !(l : A list) r.
-     dest l r =
-       let (b,r') = rbit r in
-       if b then l else
-       let (x,r'') = d r' in
-       dest (CONS x l) r''`,
-  GEN_TAC THEN
+ (`!n w. ?loop. !r.
+     loop r =
+     let (m,r') = rdecode_uniform_dest w r in
+     if m < n then m else
+     loop r'`,
+  REPEAT GEN_TAC THEN
   MP_TAC
    (ISPECL
-      [`\ ((l : A list), (r : random)).
-          let (b,r') = rbit r in
-          ~b`;
-       `\ ((l : A list), (r : random)).
-          let (b,r') = rbit r in
-          let (x,r'') = (d : random -> A # random) r' in
-          (CONS x l, r'')`;
-       `\ ((l : A list), (r : random)).
-          l`] WF_REC_TAIL) THEN
+      [`\ (r : random).
+          let (m,r') = rdecode_uniform_dest w r in
+          ~(m < n)`;
+       `\ (r : random).
+          let (m,r') = rdecode_uniform_dest w r in
+          r'`;
+       `\ (r : random).
+          let (m,r') = rdecode_uniform_dest w r in
+          m`] WF_REC_TAIL) THEN
   DISCH_THEN
-    (X_CHOOSE_THEN `dest : A list # random -> A list`
+    (X_CHOOSE_THEN `loop : random -> num`
      STRIP_ASSUME_TAC) THEN
-  EXISTS_TAC
-    `\ (l : A list) (r : random).
-       ((dest (l,r)) : A list)` THEN
+  EXISTS_TAC `loop : random -> num` THEN
   REPEAT GEN_TAC THEN
   REWRITE_TAC [] THEN
   FIRST_X_ASSUM (fun th -> CONV_TAC (LAND_CONV (ONCE_REWRITE_CONV [th]))) THEN
   REWRITE_TAC [LET_DEF; LET_END_DEF] THEN
-  PAIR_CASES_TAC `rbit r` THEN
+  PAIR_CASES_TAC `rdecode_uniform_dest w r` THEN
   DISCH_THEN
-    (X_CHOOSE_THEN `b : bool` (X_CHOOSE_THEN `r' : random` SUBST1_TAC)) THEN
+    (X_CHOOSE_THEN `m : num` (X_CHOOSE_THEN `r' : random` SUBST1_TAC)) THEN
   REWRITE_TAC [] THEN
-  BOOL_CASES_TAC `b : bool` THENL
-  [REWRITE_TAC [];
-   REWRITE_TAC [] THEN
-   PAIR_CASES_TAC `(d : random -> A # random) r'` THEN
-   DISCH_THEN
-     (X_CHOOSE_THEN `x : A` (X_CHOOSE_THEN `r'' : random` SUBST1_TAC)) THEN
-   REWRITE_TAC []]);;
+  BOOL_CASES_TAC `m < (n : num)` THEN
+  REWRITE_TAC []);;
 
-let rdecode_list_dest_def =
-  new_specification ["rdecode_list_dest"]
-    (ONCE_REWRITE_RULE [SKOLEM_THM] rdecode_list_dest_exists);;
+let rdecode_uniform_loop_def =
+  new_specification ["rdecode_uniform_loop"]
+    (ONCE_REWRITE_RULE [SKOLEM_THM]
+      (ONCE_REWRITE_RULE [SKOLEM_THM]
+        rdecode_uniform_loop_exists));;
 
-export_thm rdecode_list_dest_def;;
+export_thm rdecode_uniform_loop_def;;
 
+(***
 let rdecode_uniform_def = new_definition
   `!n r.
      rdecode_uniform n r =
-     let w = log2_num n in
+     if n = 1 then (0,r) else
+     let w = log 2 n + 1 in
      let (r1,r2) = rsplit r in
-     (rdecode_uniform_loop n w r1, r2);;
+     (rdecode_uniform_loop n w r1 MOD n, r2)`;;
 
 export_thm rdecode_uniform_def;;
 ***)
