opentheory/haskell/char.ml
@@ -33,6 +33,12 @@ let unicodeH_tybij = define_haskell_type
 
 export_thm unicodeH_tybij;;
 
+let equal_planeH_def = new_definition
+  `equal_planeH = ((=) : planeH -> planeH -> bool)`;;
+
+add_haskell_thm equal_planeH_def;;
+export_thm equal_planeH_def;;
+
 let mk_planeH_def = define_haskell_const
   `mk_plane : byte -> plane`;;
 
@@ -42,6 +48,17 @@ let dest_planeH_def = define_haskell_const
   `dest_plane : plane -> byte`;;
 
 export_thm dest_planeH_def;;
+
+let rdecode_planeH_def = define_haskell_const
+  `rdecode_plane : random -> plane # random`;;
+
+export_thm rdecode_planeH_def;;
+
+let equal_positionH_def = new_definition
+  `equal_positionH = ((=) : positionH -> positionH -> bool)`;;
+
+add_haskell_thm equal_positionH_def;;
+export_thm equal_positionH_def;;
 
 let mk_positionH_def = define_haskell_const
   `mk_position : word16 -> position`;;
@@ -53,6 +70,17 @@ let dest_positionH_def = define_haskell_const
 
 export_thm dest_positionH_def;;
 
+let rdecode_positionH_def = define_haskell_const
+  `rdecode_position : random -> position # random`;;
+
+export_thm rdecode_positionH_def;;
+
+let equal_unicodeH_def = new_definition
+  `equal_unicodeH = ((=) : unicodeH -> unicodeH -> bool)`;;
+
+add_haskell_thm equal_unicodeH_def;;
+export_thm equal_unicodeH_def;;
+
 let mk_unicodeH_def = define_haskell_const
   `mk_unicode : plane # position -> unicode`;;
 
@@ -62,6 +90,11 @@ let dest_unicodeH_def = define_haskell_const
   `dest_unicode : unicode -> plane # position`;;
 
 export_thm dest_unicodeH_def;;
+
+let rdecode_unicodeH_def = define_haskell_const
+  `rdecode_unicode : random -> unicode # random`;;
+
+export_thm rdecode_unicodeH_def;;
 
 (* UTF-8 encoding *)
 
@@ -129,16 +162,85 @@ logfile "haskell-char-src";;
 (* Unicode characters *)
 
 let () = (export_haskell_thm o prove)
- (`!p : planeH. mk_planeH (dest_planeH p) = p`,
+ (`!p. mk_planeH (dest_planeH p) = p`,
   HASKELL_TAC [plane_tybij]);;
 
 let () = (export_haskell_thm o prove)
- (`!p : positionH. mk_positionH (dest_positionH p) = p`,
+ (`!p1 p2. equal_planeH p1 p2 = (dest_planeH p1 = dest_planeH p2)`,
+  HASKELL_TAC [dest_plane_inj]);;
+
+let () = (export_haskell_thm o prove)
+ (`!r.
+     rdecode_planeH r =
+     let (n,r') = rdecode_uniformH 17 r in
+     (mk_planeH (num_to_byte n), r')`,
+  GEN_TAC THEN
+  HASKELL_TAC [rdecode_plane_def] THEN
+  PAIR_CASES_TAC `rdecode_uniform 17 r` THEN
+  DISCH_THEN
+    (X_CHOOSE_THEN `n : num`
+      (X_CHOOSE_THEN `r' : random` STRIP_ASSUME_TAC)) THEN
+  ASM_REWRITE_TAC [rdecode_plane_def; LET_DEF; LET_END_DEF] THEN
+  HASKELL_TAC []);;
+
+let () = (export_haskell_thm o prove)
+ (`!p. mk_positionH (dest_positionH p) = p`,
   HASKELL_TAC [position_tybij]);;
 
 let () = (export_haskell_thm o prove)
- (`!c : unicodeH. mk_unicodeH (dest_unicodeH p) = p`,
+ (`!p1 p2. equal_positionH p1 p2 = (dest_positionH p1 = dest_positionH p2)`,
+  HASKELL_TAC [dest_position_inj]);;
+
+(***
+let () = (export_haskell_thm o prove)
+ (`!r.
+     rdecode_positionH r =
+     let (w,r') = rdecode_word16H r in
+     (mk_positionH w, r')`,
+  GEN_TAC THEN
+  HASKELL_TAC [rdecode_plane_def] THEN
+  PAIR_CASES_TAC `rdecode_uniform 17 r` THEN
+  DISCH_THEN
+    (X_CHOOSE_THEN `n : num`
+      (X_CHOOSE_THEN `r' : random` STRIP_ASSUME_TAC)) THEN
+  ASM_REWRITE_TAC [rdecode_plane_def; LET_DEF; LET_END_DEF] THEN
+  HASKELL_TAC []);;
+***)
+
+let () = (export_haskell_thm o prove)
+ (`!c. mk_unicodeH (dest_unicodeH c) = c`,
   HASKELL_TAC [unicode_tybij]);;
+
+let () = (export_haskell_thm o prove)
+ (`!c1 c2.
+     equal_unicodeH c1 c2 =
+     let (pl1,pos1) = dest_unicodeH c1 in
+     let (pl2,pos2) = dest_unicodeH c2 in
+     equal_planeH pl1 pl2 /\ equal_positionH pos1 pos2`,
+  REPEAT GEN_TAC THEN
+  HASKELL_TAC [] THEN
+  MP_TAC (SPEC `destH_unicodeH c1` dest_unicode_cases) THEN
+  STRIP_TAC THEN
+  MP_TAC (SPEC `destH_unicodeH c2` dest_unicode_cases) THEN
+  STRIP_TAC THEN
+  ASM_REWRITE_TAC [LET_DEF; LET_END_DEF] THEN
+  HASKELL_TAC [] THEN
+  REWRITE_TAC [GSYM PAIR_EQ] THEN
+  EQ_TAC THENL
+  [POP_ASSUM (K ALL_TAC) THEN
+   POP_ASSUM (K ALL_TAC) THEN
+   POP_ASSUM (MP_TAC o REWRITE_RULE [unicode_rep_abs]) THEN
+   DISCH_THEN
+     (fun th -> CONV_TAC (RAND_CONV (ONCE_REWRITE_CONV [GSYM th]))) THEN
+   POP_ASSUM (K ALL_TAC) THEN
+   POP_ASSUM (K ALL_TAC) THEN
+   POP_ASSUM (MP_TAC o REWRITE_RULE [unicode_rep_abs]) THEN
+   DISCH_THEN
+     (fun th -> CONV_TAC (RAND_CONV (ONCE_REWRITE_CONV [GSYM th]))) THEN
+   STRIP_TAC THEN
+   ASM_REWRITE_TAC [];
+   STRIP_TAC THEN
+   ASM_REWRITE_TAC []]);;
 
 (* UTF-8 encoding *)
 
@@ -146,11 +248,35 @@ let () = (export_haskell_thm o prove)
 (* Testing.                                                                  *)
 (* ------------------------------------------------------------------------- *)
 
-(***
 logfile "haskell-char-test";;
 
 (* Unicode characters *)
 
+let () = (export_haskell_thm o prove)
+ (`!r.
+     let (c,r') = rdecode_unicodeH r in
+     let (pl,pos) = dest_unicodeH c in
+     let pli = dest_planeH pl in
+     let posi = dest_positionH pos in
+     ~(pli = num_to_byte 0) \/
+     word16_lt posi (num_to_word16 55296) \/
+     (word16_lt (num_to_word16 57343) posi /\
+      word16_lt posi (num_to_word16 65534))`,
+  GEN_TAC THEN
+  PAIR_CASES_TAC `rdecode_unicodeH r` THEN
+  DISCH_THEN
+    (X_CHOOSE_THEN `c : unicodeH`
+      (X_CHOOSE_THEN `r' : random` STRIP_ASSUME_TAC)) THEN
+  ASM_REWRITE_TAC [LET_DEF; LET_END_DEF] THEN
+  HASKELL_TAC [] THEN
+  MP_TAC (SPEC `destH_unicodeH c` dest_unicode_cases) THEN
+  STRIP_TAC THEN
+  ASM_REWRITE_TAC [] THEN
+  HASKELL_TAC [] THEN
+  UNDISCH_TAC `is_unicode (pl,pos)` THEN
+  REWRITE_TAC [is_unicode_def; LET_DEF; LET_END_DEF]);;
+
+(***
 (* UTF-8 encoding *)
 ***)
 
